proper APIs of alpha function

src/etv/alpha_beta.lean
@@ -8,33 +8,135 @@ variables
   {α : Type*} [linear_order α] {C : config α} 
   {S : finset α} (l : C.label S)
 
-private lemma mem_imply_nnil {α : Type*} (a : α) {l : list α} (ha : a ∈ l) : l ≠ [] := 
+private lemma mem_imply_nnil 
+  {α : Type*} (a : α) {l : list α} (ha : a ∈ l) : l ≠ [] := 
   by intro eq; subst eq; simp at ha; tauto
 
 namespace config.label
 
 def is_alpha_cup (a : α) (c : list α) : Prop :=
-  (c ++ [a]).in S ∧ (c ++ [a]).chain' l.slopeᶜ
+  (c ++ [a]).in S ∧ (c ++ [a]).sorted (<) ∧ (c ++ [a]).chain' l.slopeᶜ
 
 instance decidable_is_alpha_cup (a : α) (c : list α) :
   decidable (l.is_alpha_cup a c) := by rw is_alpha_cup; apply_instance
 
+theorem alpha_cup_is_cup {c : list α} 
+  (c_in_S : c.in S) (c_sorted : c.sorted (<))
+  (c_chain : c.chain' l.slopeᶜ) : C.cup c :=
+begin
+  induction c with h0 c ih, simp,
+  cases c with h1 c, simp,
+  cases c with h2 c,
+  { simp, simp at c_sorted, assumption, },
+  simp, refine ⟨_, _, _⟩,
+  simp at c_sorted; tauto,
+  simp at c_in_S c_chain c_sorted; apply l.extend_left; tauto,
+  apply ih; simp at ⊢ c_in_S c_chain c_sorted; tauto,
+end
+
+def alpha_cups' (a : α) : list (list α) :=
+  (S.sort (≤)).sublists.filter (l.is_alpha_cup a)
+
 def alpha_cup' (a : α) : option (list α) :=
-  ((S.sort (≤)).sublists.filter (l.is_alpha_cup a)).argmax list.length
+  (l.alpha_cups' a).argmax list.length
 
 def alpha_cup'_is_some {a : α} (ha : a ∈ S) : 
   option.is_some (l.alpha_cup' a) :=
 begin
   rw [←option.ne_none_iff_is_some, config.label.alpha_cup'], simp,
-  apply mem_imply_nnil [], simp [config.label.is_alpha_cup], exact ha,
+  apply mem_imply_nnil [], simp [is_alpha_cup, alpha_cups'], exact ha,
 end
-
-def alpha_cup {a : α} (ha : a ∈ S) : list α :=
-  option.get (l.alpha_cup'_is_some ha)
 
 -- one off from actual definition
 def alpha (a : α) : ℕ := 
-  if ha : a ∈ S then (l.alpha_cup ha).length else 0
+  if ha : a ∈ S then (option.get (l.alpha_cup'_is_some ha)).length else 0
+
+-- APIs for alpha: First, existence of a cup with length alpha + 1
+def alpha_cup {a : α} (ha : a ∈ S) : 
+  Σ' c : list α, c.length = l.alpha a + 1 ∧ 
+    c.in S ∧ c.sorted (<) ∧ c.chain' l.slopeᶜ ∧ a ∈ c.last' :=
+begin
+  have some := l.alpha_cup'_is_some ha,
+  set c := option.get some with def_c, 
+  rw alpha, rw dif_pos ha, rw ←def_c,
+  have h_argmax := option.get_mem some, 
+  rw [←def_c, alpha_cup'] at h_argmax,
+  have c_alpha_cup := list.argmax_mem h_argmax,
+  simp [alpha_cups', is_alpha_cup] at c_alpha_cup,
+  use (c ++ [a]), simp, tauto,
+end
+
+-- Next, maximality of the cup with length alpha + 1
+def cup_length_le_alpha {a : α} {c : list α}
+  (c_in_S : c.in S) 
+  (c_sorted : c.sorted (<))
+  (c_chain : c.chain' l.slopeᶜ)
+  (c_last : a ∈ c.last') : c.length ≤ l.alpha a + 1 :=
+begin
+  have ha : a ∈ S := c_in_S _ (list.mem_of_mem_last' c_last),
+  have some := l.alpha_cup'_is_some ha,
+  set d := option.get some with def_d, 
+  rw alpha, rw dif_pos ha, rw ←def_d,
+  have h_argmax := option.get_mem some, 
+  rw [←def_d, alpha_cup'] at h_argmax,
+  rcases list.take_last' c_last with ⟨c', eq_c⟩,
+  subst eq_c, simp,
+  have c'_alpha_cup : c' ∈ l.alpha_cups' a := begin
+    rw alpha_cups', simp, split,
+    { apply list.sublist_of_subperm_of_sorted _ _ 
+        (finset.sort_sorted_lt S),
+      apply list.nodup.subperm,
+      apply @list.nodup.sublist _ _ (c' ++ [a]), 
+      simp, exact (list.sorted.nodup c_sorted),
+      intros a ha, simp, simp at c_in_S, exact (c_in_S.left) _ ha,
+      apply list.pairwise.sublist _ c_sorted, simp, },
+    { refine ⟨_, _, _⟩; assumption },
+  end,
+  exact list.le_of_mem_argmax c'_alpha_cup h_argmax,
+end
+
+theorem add_alpha {a : α} (ha : a ∈ S)
+  {n : ℕ} {c : list α} (c_in_S : c.in S)
+  (c_cup : C.ncup n c) (c_head : a ∈ c.head') : 
+  C.has_ncup (n + l.alpha a) S :=
+begin
+  rcases (l.alpha_cup ha) with 
+    ⟨d, d_length, d_in_S, d_sorted, d_chain, d_last⟩,
+  have d_cup : C.cup d := l.alpha_cup_is_cup d_in_S d_sorted d_chain,
+  rcases list.take_last' d_last with ⟨d', eq_d⟩,
+  rcases list.take_head' c_head with ⟨c', eq_c⟩,
+  use d' ++ a :: c', 
+  by_cases hd' : d' = [],
+  { subst hd', simp at eq_d, subst eq_d, simp at d_length, rw d_length,
+    rw ←eq_c, split; simp; assumption, },
+  rcases list.take_last hd' with ⟨p, d'', eq_d'⟩,
+  cases c' with q c'',
+  { subst eq_c, cases c_cup with _ c_len, simp at c_len,
+    subst c_len, rw ←eq_d, refine ⟨⟨_, _⟩, _⟩,
+    assumption, rw d_length, exact add_comm _ _, assumption, },
+  rw eq_d', split, 
+  { rw [config.ncup], split, simp, refine ⟨_, _, _⟩,
+    convert d_cup, rw [eq_d, eq_d'], simp,
+    rw eq_d' at eq_d, simp at eq_d, 
+    rw eq_d at d_chain d_sorted d_in_S,
+    rw eq_c at c_in_S c_cup,
+    rw list.sorted at d_sorted,
+    rw [config.ncup, config.cup] at c_cup,
+    apply l.extend_left,
+    simp at d_in_S; tauto, simp at d_in_S; tauto,
+    have t := @list.pairwise.sublist 
+      _ _ [p, a] (d'' ++ [p, a]) _ d_sorted,
+    simp at t, exact t, simp,
+    simp at d_chain; tauto,
+    simp at c_in_S; tauto,
+    simp at c_cup; tauto,
+    rw ←eq_c, exact c_cup.left,
+    rw eq_d at d_length, simp at d_length,
+    rw ←eq_c, rw ←eq_d', simp, rw d_length,
+    rw c_cup.right, exact add_comm _ _, },
+  { rw ←eq_c, rw ←eq_d', simp, rw eq_d at d_in_S,
+    simp at d_in_S, tauto, },
+end
 
 end config.label
 
